An important change in the `regional` typeclass: now `Rgl?.r_repr` requires `Rgl?.r_inv`; this is necessary for correctness proofs

secure_api/merkle_tree/Low.Regional.Instances.fst
@@ -1,4 +1,4 @@
-module Low.RVector.Instances
+module Low.Regional.Instances
 
 open FStar.All
 open FStar.Integers
@@ -25,13 +25,6 @@ let buffer_region_of #a v =
 val buffer_dummy: a:Type -> Tot (B.buffer a)
 let buffer_dummy _ = B.null
 
-val buffer_repr: a:Type0 -> Type0
-let buffer_repr a = S.seq a
-
-val buffer_r_repr:
-  #a:Type -> h:HS.mem -> v:B.buffer a -> GTot (buffer_repr a)
-let buffer_r_repr #a h v = B.as_seq h v
-
 val buffer_r_inv:
   #a:Type -> len:UInt32.t{len > 0ul} ->
   h:HS.mem -> v:B.buffer a -> GTot Type0
@@ -46,6 +39,15 @@ val buffer_r_inv_reg:
 	(ensures (MHS.live_region h (buffer_region_of v)))
 let buffer_r_inv_reg #a len h v = ()
 
+val buffer_repr: a:Type0 -> len:nat{len > 0} -> Type0
+let buffer_repr a len = s:S.seq a{S.length s = len}
+
+val buffer_r_repr:
+  #a:Type -> len:UInt32.t{len > 0ul} ->
+  h:HS.mem -> v:B.buffer a{buffer_r_inv len h v} -> 
+  GTot (buffer_repr a (UInt32.v len))
+let buffer_r_repr #a len h v = B.as_seq h v
+
 val buffer_r_sep:
   #a:Type -> len:UInt32.t{len > 0ul} ->
   v:B.buffer a -> p:loc -> h0:HS.mem -> h1:HS.mem ->
@@ -55,7 +57,7 @@ val buffer_r_sep:
 		      (buffer_region_of v)) p /\
 		  modifies p h0 h1))
 	(ensures (buffer_r_inv len h1 v /\
-		 buffer_r_repr h0 v == buffer_r_repr h1 v))
+		 buffer_r_repr len h0 v == buffer_r_repr len h1 v))
 let buffer_r_sep #a len v p h0 h1 =
   assert (loc_includes (loc_all_regions_from false (buffer_region_of v))
 		       (loc_buffer v));
@@ -63,7 +65,7 @@ let buffer_r_sep #a len v p h0 h1 =
 
 val buffer_irepr: 
   #a:Type0 -> ia:a -> len:UInt32.t{len > 0ul} ->
-  Ghost.erased (buffer_repr a)
+  Ghost.erased (buffer_repr a (UInt32.v len))
 let buffer_irepr #a ia len =
   Ghost.hide (S.create (UInt32.v len) ia)
 
@@ -83,7 +85,7 @@ val buffer_r_init:
       buffer_r_init_p v /\
       buffer_r_inv len h1 v /\
       buffer_region_of v = r /\
-      buffer_r_repr h1 v == Ghost.reveal (buffer_irepr ia len)))
+      buffer_r_repr len h1 v == Ghost.reveal (buffer_irepr ia len)))
 let buffer_r_init #a ia len r =
   B.malloc r ia len
 
@@ -107,7 +109,7 @@ val buffer_copy:
     (ensures (fun h0 _ h1 ->
       modifies (loc_all_regions_from false (buffer_region_of dst)) h0 h1 /\
       buffer_r_inv len h1 dst /\
-      buffer_r_repr h1 dst == buffer_r_repr h0 src))
+      buffer_r_repr len h1 dst == buffer_r_repr len h0 src))
 let buffer_copy #a len src dst =
   B.blit src 0ul dst 0ul len
 
@@ -117,10 +119,10 @@ val buffer_regional:
 let buffer_regional #a ia len =
   Rgl (buffer_region_of #a)
       (buffer_dummy a)
-      (buffer_repr a)
-      (buffer_r_repr #a)
       (buffer_r_inv #a len)
       (buffer_r_inv_reg #a len)
+      (buffer_repr a (UInt32.v len))
+      (buffer_r_repr #a len)
       (buffer_r_sep #a len)
       (buffer_irepr #a ia len)
       (buffer_r_init_p #a)
@@ -143,18 +145,10 @@ val vector_dummy:
   #a:Type -> rg:regional a -> Tot (rvector rg)
 let vector_dummy #a rg = V.create_empty a
 
-val vector_repr: #a:Type0 -> rg:regional a -> Tot Type0
-let vector_repr #a rg = S.seq (Rgl?.repr rg)
-
-val vector_r_repr:
-  #a:Type -> #rg:regional a -> h:HS.mem -> v:rvector rg ->
-  GTot (vector_repr rg)
-let vector_r_repr #a #rg h v = RV.as_seq h v
-
 val vector_r_inv:
   #a:Type -> #rg:regional a -> 
   h:HS.mem -> v:rvector rg -> GTot Type0
-let vector_r_inv #a #rg h v = rv_inv h v
+let vector_r_inv #a #rg h v = RV.rv_inv h v
 
 val vector_r_inv_reg:
   #a:Type -> #rg:regional a -> 
@@ -162,6 +156,15 @@ val vector_r_inv_reg:
   Lemma (requires (vector_r_inv h v))
 	(ensures (MHS.live_region h (vector_region_of v)))
 let vector_r_inv_reg #a #rg h v = ()    
+
+val vector_repr: #a:Type0 -> rg:regional a -> Tot Type0
+let vector_repr #a rg = S.seq (Rgl?.repr rg)
+
+val vector_r_repr:
+  #a:Type -> #rg:regional a -> 
+  h:HS.mem -> v:rvector rg{vector_r_inv h v} ->
+  GTot (vector_repr rg)
+let vector_r_repr #a #rg h v = RV.as_seq h v
 
 val vector_r_sep:
   #a:Type -> #rg:regional a ->
@@ -219,10 +222,10 @@ val vector_regional:
 let vector_regional #a rg =
   Rgl (vector_region_of #a #rg)
       (vector_dummy #a rg)
-      (vector_repr #a rg)
-      (vector_r_repr #a #rg)
       (vector_r_inv #a #rg)
       (vector_r_inv_reg #a #rg)
+      (vector_repr #a rg)
+      (vector_r_repr #a #rg)
       (vector_r_sep #a #rg)
       (vector_irepr #a rg)
       (vector_r_init_p #a #rg)
